Instantiate encoding for compartmentalization.

compartmentalization/main.v
@@ -1,7 +1,8 @@
-Require Import ssreflect ssrbool eqtype.
+Require Import ZArith.
 
-Require Import lib.Coqlib.
-Require Import lib.utils.
+Require Import ssreflect ssrfun ssrbool eqtype fintype seq finset.
+
+Require Import lib.utils lib.partial_maps lib.Coqlib lib.Integers.
 Require Import common.common.
 Require Import concrete.concrete.
 Require Import concrete.int_32.
@@ -15,6 +16,12 @@ Require Import compartmentalization.symbolic.
 Require Import compartmentalization.abstract.
 Require Import compartmentalization.refinementSA.
 
+Import DoNotation.
+
+Set Implicit Arguments.
+Unset Strict Implicit.
+Unset Printing Implicit Defensive.
+
 Section Refinement.
 
 Let t := concrete_int_32_t.
@@ -23,8 +30,146 @@ Existing Instance concrete_int_32_ops.
 Existing Instance concrete_int_32_ops_spec.
 Existing Instance sp.
 
-Context {enc : encodable t (@Sym.stags t)}
-        {monitor_invariant : kernel_invariant}
+Definition read_kernel_word (mem : Concrete.memory t) (addr : word t) : option (word t) :=
+  do! x <- PartMaps.get mem addr;
+  if Concrete.is_kernel_tag (common.tag x) then Some (common.val x)
+  else None.
+
+Lemma read_kernel_word_monotonic mem mem' addr x ct x' ct' :
+  PartMaps.get mem addr = Some x@ct ->
+  ~~ Concrete.is_kernel_tag ct ->
+  PartMaps.upd mem addr x'@ct' = Some mem' ->
+  ~~ Concrete.is_kernel_tag ct' ->
+  read_kernel_word mem' =1 read_kernel_word mem.
+Proof.
+  move=> Hget Hnk Hupd Hnk' addr'.
+  rewrite /read_kernel_word (PartMaps.get_upd Hupd).
+  have [-> {addr'} /=|//] := altP (addr' =P addr).
+  by rewrite Hget /= (negbTE Hnk) (negbTE Hnk').
+Qed.
+
+Fixpoint read_kernel_array (mem : Concrete.memory t) (addr : word t) (count : nat) : option (seq.seq (word t)) :=
+  match count with
+  | 0 => Some [::]
+  | S count =>
+    do! x <- read_kernel_word mem addr;
+    do! arr <- read_kernel_array mem (addr + 1)%w count;
+    Some (x :: arr)
+  end.
+
+Lemma read_kernel_array_monotonic mem mem' addr x ct x' ct' :
+  PartMaps.get mem addr = Some x@ct ->
+  ~~ Concrete.is_kernel_tag ct ->
+  PartMaps.upd mem addr x'@ct' = Some mem' ->
+  ~~ Concrete.is_kernel_tag ct' ->
+  read_kernel_array mem =2 read_kernel_array mem'.
+Proof.
+  move=> Hget Hnk Hupd Hnk' addr' count.
+  elim: count addr' => [|count IH] addr' //=.
+  by rewrite (read_kernel_word_monotonic Hget Hnk Hupd Hnk') IH.
+Qed.
+
+Definition read_set (mem : Concrete.memory t) (addr : word t) : option {set word t} :=
+  do! count <- PartMaps.get mem addr;
+  if Concrete.is_kernel_tag (common.tag count) then
+    omap (fun arr => [set x : [finType of word t] in arr])
+         (read_kernel_array mem (addr + 1)%w (Z.to_nat (Word.unsigned (common.val count))))
+  else
+    None.
+
+Lemma read_set_monotonic mem mem' addr x ct x' ct' :
+  PartMaps.get mem addr = Some x@ct ->
+  ~~ Concrete.is_kernel_tag ct ->
+  PartMaps.upd mem addr x'@ct' = Some mem' ->
+  ~~ Concrete.is_kernel_tag ct' ->
+  read_set mem =1 read_set mem'.
+Proof.
+  move=> Hget Hnk Hupd Hnk' addr'.
+  rewrite /read_set (PartMaps.get_upd Hupd).
+  have [-> {addr'} /=|_] := altP (addr' =P addr).
+    by rewrite Hget /= (negbTE Hnk) (negbTE Hnk').
+  case: (PartMaps.get mem addr') => [count|] //=.
+  by rewrite (read_kernel_array_monotonic Hget Hnk Hupd Hnk').
+Qed.
+
+Definition decode_reg_tag (mem : Concrete.memory t) (tg : word t) : option (tag unit) :=
+  let: [wu ut; w']%w := Word.unpack [:: 29; 1] tg in
+  if w' == Word.one then
+    if ut == Word.zero then Some (USER tt)
+    else None
+  else None.
+
+Definition decode_data_tag (mem : Concrete.memory t) (tg : word t) : option (tag (Sym.data_tag t)) :=
+  let: [wu ut; w']%w := Word.unpack [:: 29; 1] tg in
+  if w' == Word.zero then None
+  else if (w' == Word.one) || (w' == Word.repr 2) then
+    let addr : word t := Word.castu ut in
+    do! cid <- read_kernel_word mem addr;
+    do! Iaddr <- read_kernel_word  mem (addr + 1)%w;
+    do! I <- read_set mem Iaddr;
+    do! Waddr <- read_kernel_word mem (addr + 2)%w;
+    do! W <- read_set mem Waddr;
+    let tg := Sym.DATA cid I W in
+    if w' == Word.one then Some (USER tg)
+    else Some (ENTRY tg)
+  else None.
+
+Lemma decode_data_tag_user_inv mem tg ut :
+  decode_data_tag mem tg = Some (USER ut) ->
+  ~~ Concrete.is_kernel_tag tg.
+Proof.
+  move=> Hdec.
+  apply/negP => /eqP E.
+  by rewrite {}E {tg} in Hdec.
+Qed.
+
+Definition decode_pc_tag (mem : Concrete.memory t) (tg : word t) : option (tag (Sym.pc_tag t)) :=
+  let: [wu ut; w']%w := Word.unpack [:: 29; 1] tg in
+  if w' == Word.zero then None
+  else if (w' == Word.one) || (w' == Word.repr 2) then
+    let: [wu wf; cid_addr]%w := Word.unpack [:: 0; 28] ut in
+    let wf := if wf == Word.zero then INTERNAL
+              else JUMPED in
+    let cid_addr := Word.castu cid_addr in
+    do! cid <- read_kernel_word mem cid_addr;
+    let tg := Sym.PC wf cid in
+    if w' == Word.one then Some (USER tg)
+    else Some (ENTRY tg)
+  else None.
+
+Instance encodable_stags : encodable t (@Sym.stags t) := {
+  decode tk mem tg :=
+    match tk with
+    | Symbolic.R => decode_reg_tag mem tg
+    | Symbolic.M => decode_data_tag mem tg
+    | Symbolic.P => decode_pc_tag mem tg
+    end
+}.
+Proof.
+  - move=> mem mem' addr x y ct st ct' st' [] //.
+    + move=> Hget /decode_data_tag_user_inv Hnk Hupd
+                  /decode_data_tag_user_inv Hnk' addr'.
+      rewrite /decode_data_tag.
+      case: (Word.unpack _ _) => [ut [w' []]].
+      case: (w' == 0%w) => //.
+      case: (_ || _) => //.
+      rewrite !(read_kernel_word_monotonic Hget Hnk Hupd Hnk').
+      case: (read_kernel_word _ (Word.castu ut + 1)%w) => [Iaddr|] //=.
+      rewrite (read_set_monotonic Hget Hnk Hupd Hnk').
+      case: (read_kernel_word _ (Word.castu ut + 2)%w) => [Waddr|] //=.
+      by rewrite (read_set_monotonic Hget Hnk Hupd Hnk').
+    + move=> Hget /decode_data_tag_user_inv Hnk Hupd
+                  /decode_data_tag_user_inv Hnk' addr'.
+      rewrite /decode_pc_tag.
+      case: (Word.unpack _ _) => [ut [w' []]].
+      case: (w' == 0%w) => //.
+      case: (_ || _) => //.
+      case: (Word.unpack _ _) => [wf [cid_addr []]].
+      by rewrite (read_kernel_word_monotonic Hget Hnk Hupd Hnk').
+  - by case.
+Qed.
+
+Context {monitor_invariant : kernel_invariant}
         {syscall_addrs : compartmentalization_syscall_addrs t}.
 
 Inductive refine_state (ast : Abs.state t) (cst : Concrete.state t) : Prop :=
